src/lib/state/DY.Lib.State.PrivateKeys.fst
@@ -46,16 +46,20 @@ instance map_types_private_keys: map_types private_key_key private_key_value = {
   ps_value_t = ps_private_key_value;
 }
 
+val long_term_key_label: principal -> label
+let long_term_key_label prin =
+  principal_tag_label prin "DY.Lib.State.PrivateKeys"
+
 val is_private_key_for:
   {|crypto_invariants|} -> trace ->
   bytes -> private_key_type -> principal -> prop
 let is_private_key_for #cinvs tr sk sk_type who =
   match sk_type with
   | PkDec usg -> (
-    is_decryption_key (PkKey usg empty) (principal_tag_label who "DY.Lib.State.PrivateKeys") tr sk
+    is_decryption_key (PkKey usg empty) (long_term_key_label who) tr sk
   )
   | Sign usg -> (
-    is_signature_key (SigKey usg empty) (principal_tag_label who "DY.Lib.State.PrivateKeys") tr sk
+    is_signature_key (SigKey usg empty) (long_term_key_label who) tr sk
   )
 
 // The `#_` at the end is a workaround for FStarLang/FStar#3286
@@ -94,7 +98,7 @@ let initialize_private_keys = initialize_map private_key_key private_key_value #
 [@@ "opaque_to_smt"]
 val generate_private_key: principal -> state_id -> private_key_type -> traceful (option unit)
 let generate_private_key prin sess_id sk_type =
-  let* sk = mk_rand (private_key_type_to_usage sk_type) (principal_tag_label prin "DY.Lib.State.PrivateKeys") 64 in //TODO
+  let* sk = mk_rand (private_key_type_to_usage sk_type) (long_term_key_label prin) 64 in //TODO
   add_key_value prin sess_id ({ty = sk_type}) ({private_key = sk;})
 
 [@@ "opaque_to_smt"]
