examples/nsl_pk/DY.Example.NSL.Protocol.Total.Proof.fst
@@ -24,7 +24,7 @@ let crypto_predicates_nsl = {
   pkenc_pred = {
     pred = (fun tr pk msg ->
       get_sk_usage pk == PkKey "NSL.PublicKey" empty /\
-      (exists prin. get_sk_label tr pk == long_term_decryption_key_label prin /\ (
+      (exists prin. get_sk_label tr pk == long_term_key_label prin /\ (
         match parse message msg with
         | Some (Msg1 msg1) -> (
           let (alice, bob) = (msg1.alice, prin) in
@@ -69,19 +69,19 @@ val compute_message1_proof:
     // From random generation
     is_secret (join (nsl_nonce_label alice) (nsl_nonce_label bob)) tr n_a  /\
     // From random generation
-    is_secret (long_term_decryption_key_label alice) tr nonce /\
+    is_secret (long_term_key_label alice) tr nonce /\
     // From random generation
     PkNonce? (get_usage nonce) /\
     // From PKI invariants
-    is_encryption_key (PkKey "NSL.PublicKey" empty) (long_term_decryption_key_label bob) tr pk_b
+    is_encryption_key (PkKey "NSL.PublicKey" empty) (long_term_key_label bob) tr pk_b
   )
   (ensures is_publishable tr (compute_message1 alice bob pk_b n_a nonce))
 let compute_message1_proof tr alice bob pk_b n_a nonce =
   let msg = Msg1 {n_a; alice;} in
   assert(join (nsl_nonce_label alice) (nsl_nonce_label bob) `can_flow tr` (nsl_nonce_label alice));
   assert(join (nsl_nonce_label alice) (nsl_nonce_label bob) `can_flow tr` (nsl_nonce_label bob));
-  serialize_wf_lemma message (is_knowable_by (long_term_decryption_key_label alice) tr) msg;
-  serialize_wf_lemma message (is_knowable_by (long_term_decryption_key_label bob) tr) msg
+  serialize_wf_lemma message (is_knowable_by (long_term_key_label alice) tr) msg;
+  serialize_wf_lemma message (is_knowable_by (long_term_key_label bob) tr) msg
 
 // If bob successfully decrypt the first message,
 // then n_a is knownable both by alice (in the message) and bob (the principal)
@@ -95,7 +95,7 @@ val decode_message1_proof:
   Lemma
   (requires
     // From PrivateKeys invariants
-    is_decryption_key (PkKey "NSL.PublicKey" empty) (long_term_decryption_key_label bob) tr sk_b /\
+    is_decryption_key (PkKey "NSL.PublicKey" empty) (long_term_key_label bob) tr sk_b /\
     // From the network
     bytes_invariant tr msg_cipher
   )
@@ -107,7 +107,7 @@ val decode_message1_proof:
     )
   ))
 let decode_message1_proof tr bob msg_cipher sk_b =
-  assume(forall p. (long_term_decryption_key_label bob) == (long_term_decryption_key_label p) ==> bob == p);
+  assume(forall p. (long_term_key_label bob) == (long_term_key_label p) ==> bob == p);
   match decode_message1 bob msg_cipher sk_b with
   | None -> ()
   | Some msg1 ->
@@ -128,11 +128,11 @@ val compute_message2_proof:
     // From the random generation
     is_secret (join (nsl_nonce_label msg1.alice) (nsl_nonce_label bob)) tr n_b /\
     // From the random generation
-    is_secret (long_term_decryption_key_label bob) tr nonce /\
+    is_secret (long_term_key_label bob) tr nonce /\
     // From the random generation
     PkNonce? (get_usage nonce) /\
     // From the PKI
-    is_encryption_key (PkKey "NSL.PublicKey" empty) (long_term_decryption_key_label msg1.alice) tr pk_a
+    is_encryption_key (PkKey "NSL.PublicKey" empty) (long_term_key_label msg1.alice) tr pk_a
   )
   (ensures
     is_publishable tr (compute_message2 bob msg1 pk_a n_b nonce)
@@ -158,7 +158,7 @@ val decode_message2_proof:
     // From the NSL state invariant
     is_secret (join (nsl_nonce_label alice) (nsl_nonce_label bob)) tr n_a /\
     // From the PrivateKeys invariant
-    is_decryption_key (PkKey "NSL.PublicKey" empty) (long_term_decryption_key_label alice) tr sk_a /\
+    is_decryption_key (PkKey "NSL.PublicKey" empty) (long_term_key_label alice) tr sk_a /\
     // From the network
     bytes_invariant tr msg_cipher
   )
@@ -174,7 +174,7 @@ val decode_message2_proof:
     )
   ))
 let decode_message2_proof tr alice bob msg_cipher sk_a n_a =
-  assume(forall p. (long_term_decryption_key_label alice) == (long_term_decryption_key_label p) ==> alice == p);
+  assume(forall p. (long_term_key_label alice) == (long_term_key_label p) ==> alice == p);
   match decode_message2 alice bob msg_cipher sk_a n_a with
   | None -> ()
   | Some msg2 -> (
@@ -194,11 +194,11 @@ val compute_message3_proof:
     // From decode_message2_proof
     is_knowable_by (join (nsl_nonce_label alice) (nsl_nonce_label bob)) tr n_b /\
     // From the random generation
-    is_secret (long_term_decryption_key_label alice) tr nonce /\
+    is_secret (long_term_key_label alice) tr nonce /\
     // From the random generation
     PkNonce? (get_usage nonce) /\
     // From the PKI
-    is_encryption_key (PkKey "NSL.PublicKey" empty) (long_term_decryption_key_label bob) tr pk_b
+    is_encryption_key (PkKey "NSL.PublicKey" empty) (long_term_key_label bob) tr pk_b
   )
   (ensures
     is_publishable tr (compute_message3 alice bob pk_b n_b nonce)
@@ -206,8 +206,8 @@ val compute_message3_proof:
 let compute_message3_proof tr alice bob pk_b n_b nonce =
   assert(exists alice n_a. event_triggered tr alice (Initiate2 alice bob n_a n_b));
   let msg = Msg3 {n_b;} in
-  serialize_wf_lemma message (is_knowable_by (long_term_decryption_key_label alice) tr) msg;
-  serialize_wf_lemma message (is_knowable_by (long_term_decryption_key_label bob) tr) msg;
+  serialize_wf_lemma message (is_knowable_by (long_term_key_label alice) tr) msg;
+  serialize_wf_lemma message (is_knowable_by (long_term_key_label bob) tr) msg;
   let msg3: message3 = {n_b;} in
   assert(msg3.n_b == n_b)
 
@@ -223,7 +223,7 @@ val decode_message3_proof:
     // From the NSL state invariant
     get_label tr n_b == join (nsl_nonce_label alice) (nsl_nonce_label bob) /\
     // From the PrivateKeys invariant
-    is_decryption_key (PkKey "NSL.PublicKey" empty) (long_term_decryption_key_label bob) tr sk_b /\
+    is_decryption_key (PkKey "NSL.PublicKey" empty) (long_term_key_label bob) tr sk_b /\
     // From the network
     bytes_invariant tr msg_cipher
   )
@@ -239,7 +239,7 @@ val decode_message3_proof:
     )
   ))
 let decode_message3_proof tr alice bob msg_cipher sk_b n_b =
-  assume(forall p. (long_term_decryption_key_label bob) == (long_term_decryption_key_label p) ==> bob == p);
+  assume(forall p. (long_term_key_label bob) == (long_term_key_label p) ==> bob == p);
   match decode_message3 alice bob msg_cipher sk_b n_b with
   | None -> ()
   | Some msg3 -> (
